Finished proving Lemma 3 and Theorem 1, modulo Ok related proofs. Fixed bug in SAnd1 of sub data-type.

withtop/Proofs/CoherenceBasic.v
@@ -24,9 +24,6 @@ Require Import Coq.Lists.List.
 Require Import Coq.MSets.MSetInterface.
 Require Import Coq.MSets.MSetWeakList.
 
-Print MSetInterface.
-Print MSetWeakList.
-
 Module TypingRules
        (Import VarTyp : BooleanDecidableType')
        (Import set : MSetInterface.S).
@@ -85,7 +82,7 @@ Inductive sub : PTyp -> PTyp -> Exp -> Prop :=
   | SFun : forall o1 o2 o3 o4 c1 c2, sub o3 o1 c1 -> sub o2 o4 c2 -> 
      sub (Fun o1 o2) (Fun o3 o4) (STLam _ (ptyp2styp (Fun o1 o2)) (STLam _ (ptyp2styp o3) (STApp _ (c2) (STApp _ (STBVar _ 1) (STApp _ (c1) (STBVar _ 0))))))
   | SAnd1 : forall t t1 t2 c1 c2, sub t t1 c1 -> sub t t2 c2 -> 
-     sub t (And  t1 t2) (STLam _ (ptyp2styp t1)
+     sub t (And  t1 t2) (STLam _ (ptyp2styp t)
        (STPair _ (STApp _ (c1) (STBVar _ 0)) (STApp _ (c2) (STBVar _ 0))))
   | SAnd2 : forall t t1 t2 c, sub t1 t c -> Atomic t ->
      sub (And  t1 t2) t (STLam _ (ptyp2styp (And t1 t2)) 
@@ -112,7 +109,7 @@ Defined.
 
 Definition sand1 : forall t t1 t2, Sub t t1 -> Sub t t2 -> Sub t (And t1 t2).
 unfold Sub. intros. destruct H. destruct H0.
-exists (STLam _ (ptyp2styp t1) (
+exists (STLam _ (ptyp2styp t0) (
        STPair _ (STApp _ (x) (STBVar _ 0)) (STApp _ (x0) (STBVar _ 0)))).
 apply SAnd1. auto. auto.
 Defined.
@@ -147,7 +144,7 @@ assert (Sub (And t0 t3) t2). apply IHt2.
 unfold Sub. exists c2. auto.
 unfold Sub in H6. destruct H6.
 unfold Sub in H7. destruct H7.
-exists (STLam _ (ptyp2styp t1) (
+exists (STLam _ (ptyp2styp (And t0 t3)) (
        STPair _ (STApp _ (x0) (STBVar _ 0)) (STApp _ (x1) (STBVar _ 0)))).
 apply SAnd1. auto. auto.
 inversion H1.
@@ -182,7 +179,7 @@ assert (Sub (And t0 t3) t2). apply IHt2.
 unfold Sub. exists c2. auto.
 unfold Sub in H6. destruct H6.
 unfold Sub in H7. destruct H7.
-exists (STLam _ (ptyp2styp t1) (
+exists (STLam _ (ptyp2styp (And t0 t3)) (
        STPair _ (STApp _ (x0) (STBVar _ 0)) (STApp _ (x1) (STBVar _ 0)))).
 apply SAnd1. auto. auto.
 inversion H1.
@@ -466,6 +463,8 @@ Definition var : Type := VarTyp.t.
 Module M := MSetWeakList.Make(VarTyp).
 Export M.
 
+Module EqFacts := BoolEqualityFacts(VarTyp).
+
 Definition vars := M.t.
 
 (* Definitions borrowed from STLC_Tutorial *)
@@ -553,8 +552,9 @@ Ltac beautify_fset V :=
   in
   go (empty : vars) V.
 
-Definition var_fresh (L : vars) := {x : var | not (In x L) }.
-
+Definition var_fresh : forall L : vars, {x : var | not (In x L) }.
+Admitted.
+  
 Ltac pick_fresh_gen L Y :=
   let Fr := fresh "Fr" in
   let L := beautify_fset L in
@@ -587,17 +587,16 @@ Ltac intros_fresh x :=
     let Fr := fresh "Fr" x2 in
     intros x2 Fr ]. 
 
-(* TODO is this necessary? if so uncomment also in apply_fresh_base*)
 Fixpoint fresh (L : vars) (n : nat) (xs : list var) : Prop :=
   match xs with
   | nil => match n with
            | 0 => True
            | S _ => False
            end
-  | (x :: xs') =>
+  | (x :: xs')%list =>
       match n with
       | 0 => False
-      | S n' => not (In x L) /\ fresh (union L (singleton x)) n' xs'
+      | S n' => (not (In x L)) /\ fresh (union L (singleton x)) n' xs'
       end
   end.
 
@@ -627,14 +626,8 @@ Fixpoint open_rec_source (k : nat) (u : PExp) (t : PExp) {struct t} : PExp  :=
 
 Definition open_source t u := open_rec_source 0 u t.
 
-(*
-Notation "{ k ~> u } t" := (open_rec_source k u t) (at level 67).
-Notation "t ^^ u" := (open_source t u) (at level 67).
-Notation "t ^ x" := (open_source t (PFVar x)).
- *)
-
 (** Target language **)
-Fixpoint open_rec {a} (k : nat) (u : SExp a) (t : SExp a) : SExp a :=
+Fixpoint open_rec (k : nat) (u : SExp var) (t : SExp var) : SExp var :=
   match t with
   | STBVar _ i => if Nat.eqb k i then u else (STBVar _ i)
   | STFVar _ x => STFVar _ x
@@ -646,7 +639,7 @@ Fixpoint open_rec {a} (k : nat) (u : SExp a) (t : SExp a) : SExp a :=
   | STProj2 _ t => STProj2 _ (open_rec k u t)
   end.
 
-Definition open {a} (t : SExp a) u := open_rec 0 u t.
+Definition open (t : SExp var) u := open_rec 0 u t.
 
 (* Functions on contexts *)
 Definition mapctx {A B} (f : A -> B) (c : context A) : context B :=
@@ -665,11 +658,12 @@ Reserved Notation "Gamma '|-' t ':' T" (at level 40).
 
 (* Typing rules of source language: Figure 2 *)
 Inductive has_type_source : (context PTyp) -> PExp -> PTyp -> (SExp var) -> Prop :=
-  | TyVar : forall Gamma x ty, List.Exists (fun a => fst a = x /\ snd a = ty) Gamma -> 
-                      has_type_source Gamma (PFVar x) ty (STFVar _ x)
+| TyVar : forall Gamma x ty,
+            (* List.Exists (fun a => fst a = x /\ snd a = ty) Gamma -> *)
+            List.In (x,ty) Gamma -> has_type_source Gamma (PFVar x) ty (STFVar _ x)
   | TyLit : forall Gamma x, has_type_source Gamma (PLit x) PInt (STLit _ x)
-  | TyLam : forall Gamma t A B L E, (forall x, not (In x L) -> 
-                                 has_type_source (extend x A Gamma) (open_source t (PFVar x)) B E) ->
+  | TyLam : forall L Gamma t A B E, (forall x, not (In x L) -> 
+                                 has_type_source (Gamma ++ ((x,A) :: nil)) (open_source t (PFVar x)) B E) ->
                            has_type_source Gamma (PLam A t) (Fun A B) (STLam _ (|A|) E) 
   | TyApp : forall Gamma A B C t1 t2 E E1 E2,
               has_type_source Gamma t1 (Fun A B) E1 ->
@@ -683,12 +677,15 @@ Inductive has_type_source : (context PTyp) -> PExp -> PTyp -> (SExp var) -> Prop
 
 (* Typing rules of STLC, inspired by STLC_Tutorial *)
 Inductive has_type_st : (context STyp) -> (SExp var) -> STyp -> Prop :=
-  | STTyVar : forall Gamma x ty, List.Exists (fun a => (fst a) = x /\ snd a = ty) Gamma ->
+| STTyVar : forall (Gamma : context STyp) x ty,
+              (*List.Exists (fun a => (fst a) = x /\ snd a = ty) Gamma ->*)
+              List.In (x,ty) Gamma -> 
                         has_type_st Gamma (STFVar _ x) ty
   | STTyLit : forall Gamma x, has_type_st Gamma (STLit _ x) STInt       
-  | STTyLam : forall L Gamma t A B, (forall x, not (In x L) -> 
-                                 has_type_st (extend x A Gamma) (open t (STFVar _ x)) B) ->
-                           has_type_st Gamma (STLam _ A t) (STFun A B)
+  | STTyLam : forall L Gamma t A B,
+                (forall x, not (In x L) -> 
+                      has_type_st (Gamma ++ ((x,A) :: nil)) (open t (STFVar _ x)) B) ->
+                has_type_st Gamma (STLam _ A t) (STFun A B)
   | STTyApp : forall Gamma A B t1 t2, has_type_st Gamma t1 (STFun A B) ->
                              has_type_st Gamma t2 A -> has_type_st Gamma (STApp _ t1 t2) B
   | STTyPair : forall Gamma A B t1 t2, has_type_st Gamma t1 A ->
@@ -706,7 +703,19 @@ Proof.
   - rewrite <- H; reflexivity.
   - rewrite <- H; reflexivity.
 Defined.  
-  
+
+Lemma in_persists : forall x ty Gamma, List.In (x, ty) Gamma -> List.In (x, |ty|) (∥ Gamma ∥).
+Proof.
+  intros.
+  induction Gamma.
+  simpl in *; assumption.
+  simpl in *.
+  inversion H.
+  subst; simpl in *.
+  auto.
+  right; apply IHGamma; auto.
+Defined.
+
 Lemma exists_persists : forall l x v,
   List.Exists (fun p : var * PTyp => (fst p) = x /\ (snd p) = v) l ->
   List.Exists (fun p : var * STyp => (fst p) = x /\ (snd p) = (|v|)) (∥ l ∥).
@@ -722,30 +731,554 @@ Proof.
   apply Exists_cons.
   auto.
 Defined.  
+
+Lemma free_vars_in :
+  forall t1 x y n, In x (fv t1) ->
+  In x (fv (open_rec n (STFVar var y) t1)).
+Proof.
+  intro t.
+  induction t; intros; try auto.
+  (* STBVar *)
+  simpl in *; inversion H.
+  (* STLam *)
+  simpl in *.
+  apply IHt; assumption.
+  (* STApp *)
+  simpl in *.
+  apply union_spec.
+  apply union_spec in H.
+  destruct H.
+  left; apply IHt1; assumption.
+  right; apply IHt2; assumption.
+  (* STPair *)
+  simpl in *.
+  apply union_spec in H.
+  apply union_spec.
+  destruct H.
+  left; apply IHt1; assumption.
+  right; apply IHt2; assumption.
+  (* STProj1 *)
+  simpl in *; apply IHt; assumption.
+  (* STProj2 *)
+  simpl in *; apply IHt; assumption.
+Defined.
+
+Inductive STTerm : Exp -> Prop :=
+  | STTerm_Var : forall x,
+      STTerm (STFVar _ x)
+  | STTerm_Lit : forall n,
+      STTerm (STLit _ n)
+  | STTerm_Lam : forall L t1 A,
+      (forall x, not (In x L) -> STTerm (open t1 (STFVar var x))) ->
+      STTerm (STLam _ A t1)
+  | STTerm_App : forall t1 t2,
+      STTerm t1 -> 
+      STTerm t2 -> 
+      STTerm (STApp _ t1 t2)
+  | STTerm_Pair : forall t1 t2,
+      STTerm t1 ->
+      STTerm t2 ->
+      STTerm (STPair _ t1 t2)
+  | STTerm_Proj1 : forall t,
+      STTerm t ->
+      STTerm (STProj1 _ t)
+  | STTerm_Proj2 : forall t,
+      STTerm t ->
+      STTerm (STProj2 _ t).
+
+Hint Constructors STTerm.
+
+Fixpoint subst (z : var) (u : Exp) (t : Exp) {struct t} : Exp :=
+  match t with
+    | STBVar _ i     => STBVar _ i
+    | STFVar _ x     => if VarTyp.eqb x z then u else (STFVar _ x)
+    | STLit _ i      => STLit _ i
+    | STLam _ A t1   => STLam _ A (subst z u t1)
+    | STApp _ t1 t2  => STApp _ (subst z u t1) (subst z u t2)
+    | STPair _ t1 t2 => STPair _ (subst z u t1) (subst z u t2)
+    | STProj1 _ t    => STProj1 _ (subst z u t)
+    | STProj2 _ t    => STProj2 _ (subst z u t)
+  end.
+
+Require Import Coq.Init.Peano.
+
+Notation "[ z ~> u ] t" := (subst z u t) (at level 68).
+Notation "{ k ~> u } t" := (open_rec k u t) (at level 67).
+Notation "t ^ x" := (open t (STFVar var x)).
+Notation "t ^^ u" := (open t u) (at level 67).
+
+Lemma subst_fresh : forall t x u, 
+  not (In x (fv t)) ->  [x ~> u] t = t.
+Proof.
+  intro t.
+  induction t; intros; auto.
+  (* Case STFVar *)
+  simpl.
+  remember (eqb a x) as H1.
+  destruct H1.
+  exfalso.
+  apply H.
+  unfold fv; simpl.
+  apply singleton_spec.
+  symmetry in HeqH1.
+  apply eqb_eq in HeqH1; symmetry; assumption.
+  reflexivity.
+  (* Case STLam *)
+  simpl in *.
+  rewrite IHt; auto.
+  (* Case STApp *)
+  simpl in *; rewrite IHt1, IHt2; auto; unfold not in *; intros;
+  apply H; apply union_spec; [ right | left ]; auto.
+  (* Case STPair *)
+  simpl in *; rewrite IHt1, IHt2; auto; unfold not in *; intros;
+  apply H; apply union_spec; [ right | left ]; auto.
+  (* Case STProj1 *)
+  simpl in *; rewrite IHt; auto.
+  (* Case STProj2 *)
+  simpl in *; rewrite IHt; auto.
+Defined.
+
+(* ********************************************************************** *)
+(** ** Proving the two axioms *)
+
+(** We first set up four lemmas, and then we can prove our two axioms. *)
+
+(** The first lemma is a technical auxiliary lemma which do not 
+    want and do not need to read. *)
+
+
+Lemma open_rec_term_core :forall t j v i u, i <> j ->
+  { j ~> v }t = { i ~> u }({ j ~> v }t) -> t = { i ~> u }t.
+Proof.
+  intro t; induction t; intros; simpl.
+  reflexivity.
+  simpl in *.
+  case_eq (Nat.eqb i n); intros.
+  case_eq (Nat.eqb j n); intros.
+  exfalso. apply H. apply Nat.eqb_eq in H1.
+  apply Nat.eqb_eq in H2. rewrite H1, H2.
+  reflexivity.
+  rewrite H2 in H0.
+  unfold open_rec in H0.
+  rewrite H1 in H0.
+  assumption.
+  reflexivity.
+  reflexivity.
+  inversion H0.
+  erewrite <- IHt.
+  reflexivity.
+  apply not_eq_S.
+  apply H.
+  apply H2.
+  inversion H0.
+  erewrite <- IHt1.
+  erewrite <- IHt2.
+  reflexivity.
+  apply H.
+  apply H3.
+  apply H.
+  apply H2.
+  inversion H0.
+  erewrite <- IHt1.
+  erewrite <- IHt2.
+  reflexivity.
+  apply H.
+  apply H3.
+  apply H.
+  apply H2.
+  inversion H0.
+  erewrite <- IHt.
+  reflexivity.
+  apply H.
+  apply H2.
+  inversion H0.
+  erewrite <- IHt.
+  reflexivity.
+  apply H.
+  apply H2.  
+Defined.
+
+(** Substitution on indices is identity on well-formed terms. *)
+
+Lemma open_rec_term : forall t u,
+  STTerm  t -> forall k, t =  { k ~> u }t.
+Proof.
+  induction 1; intros; simpl; auto.
+  pick_fresh x.
+  rewrite <- open_rec_term_core with (j := 0) (v := STFVar _ x).
+  reflexivity.
+  auto.
+  simpl.
+  unfold open in *.
+  rewrite <- H0.
+  reflexivity.
+  unfold not; intros; apply Fr; rewrite union_spec; rewrite union_spec; left; left.
+  assumption.
+  rewrite <- IHSTTerm1.
+  rewrite <- IHSTTerm2.
+  reflexivity.
+  rewrite <- IHSTTerm1.
+  rewrite <- IHSTTerm2.
+  reflexivity.
+  rewrite <- IHSTTerm.
+  reflexivity.
+  rewrite <- IHSTTerm.
+  reflexivity.
+Defined.
+
+Hint Resolve open_rec_term.
+
+(** Substitution distributes on the open operation. *)
+
+Lemma subst_open : forall x u t1 t2, STTerm u -> 
+  [x ~> u] (open t1 t2) = open ([x ~> u]t1) ([x ~> u]t2).
+Proof.
+  intros. unfold open. generalize 0.
+  induction t1; intros; simpl.
+  (* STFVar *)
+  - case_eq (eqb a x); intros.
+    rewrite <-  open_rec_term; auto.
+    simpl; reflexivity.
+  (* STFVar *)
+  - case_eq (n0 =? n); intros; auto.
+  (* STLit *)  
+  - reflexivity.
+  (* STLam *)
+  - rewrite IHt1; reflexivity.
+  (* STApp *)
+  - rewrite IHt1_1; rewrite IHt1_2; reflexivity.
+  (* STPair *)
+  - rewrite IHt1_1; rewrite IHt1_2; reflexivity.
+  (* STProj1 *)
+  - rewrite IHt1; reflexivity.
+  (* STProj2 *)
+  - rewrite IHt1; reflexivity.
+Defined.
+
+(** Substitution and open_var for distinct names commute. *)
+
+Lemma subst_open_var : forall (x y : var) u t, not (x == y) -> STTerm u ->
+  ([x ~> u] t) ^ y = [x ~> u] (t ^ y).
+Proof.
+  intros. rewrite subst_open. simpl.
+  case_eq (eqb y x); intros.
+  apply eqb_eq in H1.
+  exfalso; apply H; symmetry. assumption.
+  reflexivity.
+  assumption.
+Defined.
   
-  
+(** Opening up an abstraction of body [t] with a term [u] is the same as opening
+  up the abstraction with a fresh name [x] and then substituting [u] for [x]. *)
+
+Lemma subst_intro : forall x t u, 
+  not (In x (fv t)) -> STTerm u ->
+  open t u = [x ~> u](t ^ x).
+Proof.
+  intros.
+  rewrite subst_open; [ | assumption ].
+  rewrite subst_fresh; [ | assumption ].
+  simpl.
+  case_eq (eqb x x); intros.
+  reflexivity.
+  rewrite EqFacts.eqb_neq in H1.
+  exfalso.
+  apply H1.
+  reflexivity.
+Defined.
+
+(* ********************************************************************** *)
+(** ** Preservation of local closure *)
+
+(** The goal of this section is to set up the appropriate lemmas 
+    for proving goals of the form [term t]. First, we defined a
+    predicate capturing that a term [t] is the body of a locally
+    closed abstraction. *)
+
+Definition body t :=
+  exists L, forall x, not (In x L) -> STTerm (t ^ x).
+
+(** We then show how to introduce and eliminate [body t]. *)
+
+Lemma term_abs_to_body : forall A t1, 
+  STTerm (STLam _ A t1) -> body t1.
+Proof.
+  intros; unfold body; inversion H; subst; exists L; assumption.
+Defined.
+
+Lemma body_to_term_abs : forall A t1, 
+  body t1 -> STTerm (STLam _ A t1).
+Proof. intros. inversion H. apply_fresh STTerm_Lam as x. apply H0.
+       unfold not in *. intros; apply Fry; apply union_spec; auto.
+Defined.
+
+(* Hint Resolve term_abs_to_body body_to_term_abs. *)
+
+(** We prove that terms are stable by substitution *)
+
+Lemma subst_term : forall t z u,
+  STTerm u -> STTerm t -> STTerm ([z ~> u]t).
+Proof.
+  induction 2; simpl; auto.
+  destruct (eqb x z).
+  assumption.
+  (* Var *)
+  - apply STTerm_Var.
+  (* Lam *)
+  - apply_fresh STTerm_Lam as x.
+    rewrite subst_open_var.
+    apply H1. unfold not in *.
+    intros; apply Frx.
+    apply union_spec; left.
+    apply union_spec; left.
+    apply union_spec; left.
+    assumption.
+    unfold not in *; intros; apply Frx.
+    apply union_spec; left.
+    apply union_spec; left.
+    apply union_spec; right.
+    apply singleton_spec.
+    symmetry; assumption.
+    assumption.
+Defined.
+
+Hint Resolve subst_term.
+
+(** We prove that opening a body with a term gives a term *)
+
+Lemma open_term : forall t u,
+  body t -> STTerm u -> STTerm (open t u).
+Proof.
+  intros t u H1 H2. destruct H1. pick_fresh y.
+  rewrite union_spec in Fr.
+  rewrite union_spec in Fr.
+  assert (Ha : not (In y x)).
+  unfold not; intros; apply Fr; left; left; assumption.
+  rewrite (@subst_intro y); auto.
+Defined.
+
+Hint Resolve open_term.
+Hint Resolve singleton_spec.
+Hint Resolve union_spec.
+    
+Lemma coercions_produce_terms :
+  forall E A B, sub A B E -> STTerm E.
+Proof.
+  intros.
+  Print sub.
+  induction H.
+  (* Case SInt *)
+  - apply_fresh STTerm_Lam as x.
+    unfold open; simpl.
+    apply STTerm_Var.
+  (* Case SFun *)
+  - apply_fresh STTerm_Lam as x.
+    unfold open; simpl.
+    apply_fresh STTerm_Lam as y.
+    unfold open; simpl.
+    apply STTerm_App.
+    rewrite <-  open_rec_term; auto.
+    rewrite <- open_rec_term; auto.
+    rewrite <- open_rec_term; auto.
+    apply STTerm_App.
+    apply STTerm_Var.
+    apply STTerm_App; try auto.
+    rewrite <- open_rec_term; auto.
+    rewrite <- open_rec_term; auto.
+    rewrite <- open_rec_term; auto.
+  (* Case SAnd1 *)
+  - apply_fresh STTerm_Lam as x.
+    unfold open; simpl.
+    apply STTerm_Pair.
+    apply STTerm_App; try auto.
+    rewrite <- open_rec_term; try auto.
+    apply STTerm_App; try auto.
+    rewrite <- open_rec_term; try auto.
+  (* Case SAnd2 *)
+  - apply_fresh STTerm_Lam as x.
+    unfold open; simpl.
+    apply STTerm_App; try auto.
+    rewrite <- open_rec_term; try auto.
+  (* Case SAnd3 *)
+  - apply_fresh STTerm_Lam as x.
+    unfold open; simpl.
+    apply STTerm_App; try auto.
+    rewrite <- open_rec_term; try auto.
+Defined.
+
+Inductive ok {A} : context A -> Prop :=
+  | Ok_nil : ok nil
+  | Ok_push : forall (E : context A) (v : var) (ty : A),
+                ok E -> not (In v (dom E)) -> ok (E ++ ((v,ty) :: nil)).        
+
+Require Import Coq.Program.Equality.
+
+Lemma typing_weaken : forall G E F t T,
+   has_type_st (E ++ G) t T -> 
+   ok (E ++ F ++ G) ->
+   has_type_st (E ++ F ++ G) t T.
+Proof.
+  intros.
+  generalize dependent H0.
+  remember (E ++ G) as H'.
+  generalize dependent HeqH'.
+  generalize dependent G.
+  dependent induction H; intros.
+  subst.
+  apply STTyVar.
+  apply in_app_or in H.
+  inversion H.
+  apply in_or_app; left; assumption.
+  apply in_or_app; right; apply in_or_app; right; assumption.
+  apply STTyLit.
+  subst.
+  apply_fresh STTyLam as x.
+  unfold open in *; simpl in *.
+  unfold extend in *.
+  rewrite <- app_assoc.
+  rewrite <- app_assoc.
+  apply H0.
+  unfold not; intros; apply Frx.
+  rewrite union_spec; rewrite union_spec; rewrite union_spec; rewrite union_spec.
+  repeat left; assumption.
+  rewrite app_assoc.
+  reflexivity.
+  admit. (* TODO ok rules here *)
+  eapply STTyApp.
+  apply IHhas_type_st1; assumption.
+  apply IHhas_type_st2; assumption.
+  eapply STTyPair.
+  apply IHhas_type_st1; assumption.
+  apply IHhas_type_st2; assumption.
+  eapply STTyProj1.
+  apply IHhas_type_st; assumption.
+  eapply STTyProj2.
+  apply IHhas_type_st; assumption.
+Admitted.
+
 (* Subtyping rules produce type-correct coercions: Lemma 3 *)
 Lemma type_correct_coercions :
   forall Gamma A B E, sub A B E ->
              has_type_st Gamma E (STFun (|A|) (|B|)) .
 Proof.
   intros.
-  Print sub.
   induction H.
   (* Case SInt *)
-  simpl.
-  apply_fresh STTyLam as x.
-  simpl; apply STTyVar.
-  apply Exists_cons_hd; auto.
-
-  
+  - simpl.
+    apply_fresh STTyLam as x.
+    simpl; apply STTyVar.
+    apply in_or_app.
+    right; simpl; auto.
   (* Case SFun *)
-  apply_fresh STTyLam as x.
-  unfold open; simpl.
-  apply_fresh STTyLam as y.
-  unfold open; simpl.
-  apply STTyApp with (A := (| o2 |)). 
+  - apply_fresh STTyLam as x.
+    unfold open; simpl.
+    apply_fresh STTyLam as y.
+    unfold open; simpl.
+    apply STTyApp with (A := (| o2 |)).
+    rewrite <- open_rec_term.
+    rewrite <- open_rec_term.
+    rewrite <- app_assoc.
+    apply typing_weaken.
+    rewrite <- app_nil_r with (l := (y, | o3 |) :: nil).
+    apply typing_weaken.
+    rewrite app_nil_r.
+    assumption.
+    admit. (* TODO ok rules here *)
+    admit. (* TODO ok rules here *)
+    eapply coercions_produce_terms.
+    apply H0.
+    rewrite <- open_rec_term; eapply coercions_produce_terms; apply H0.
+    eapply STTyApp.
+    apply STTyVar.
+    apply in_or_app; left; apply in_or_app; right.
+    simpl; auto.    
+    apply STTyApp with (A := (| o3 |)).
+    rewrite <- open_rec_term.
+    rewrite <- open_rec_term.
+    rewrite <- app_assoc.
+    apply typing_weaken.
+    rewrite <- app_nil_r with (l := (y, | o3 |) :: nil).
+    apply typing_weaken.
+    rewrite app_nil_r; assumption.
+    admit. (* TODO ok rules here *)
+    admit. (* TODO ok rules here *)
+    eapply coercions_produce_terms; apply H.    
+    rewrite <- open_rec_term; eapply coercions_produce_terms; apply H.
+    apply STTyVar.
+    apply in_or_app; right; simpl; auto.
+  (* Case SAnd1 *)
+  - apply_fresh STTyLam as x.
+    unfold open; simpl.
+    apply STTyPair.
+    eapply STTyApp.
+    rewrite <- open_rec_term.
+    rewrite <- app_nil_r with (l := (x, | t0 |) :: nil).
+    apply typing_weaken.
+    rewrite app_nil_r.
+    apply IHsub1.
+    admit. (* TODO ok rules here *)
+    apply coercions_produce_terms in H.
+    assumption.
+    apply STTyVar.
+    apply in_or_app; right; simpl; auto.
+    simpl; auto.
+    rewrite <- open_rec_term.
+    eapply STTyApp.
+    rewrite <- app_nil_r with (l := (x, | t0 |) :: nil).
+    apply typing_weaken.
+    rewrite app_nil_r.
+    apply IHsub2.
+    admit. (* TODO ok rules here *)
+    apply STTyVar.
+    apply in_or_app; right; simpl; auto.
+    apply coercions_produce_terms in H0.
+    assumption.
+  (* Case SAnd2 *)
+  - apply_fresh STTyLam as x.
+    unfold open; simpl.
+    eapply STTyApp.
+    rewrite <- open_rec_term.
+    rewrite <- app_nil_r with (l := (x, STTuple (| t1 |) (| t2 |)) :: nil).
+    apply typing_weaken.
+    rewrite app_nil_r.
+    apply IHsub.
+    admit. (* TODO ok rules here *)
+    apply coercions_produce_terms in H.
+    assumption.
+    eapply STTyProj1.
+    apply STTyVar.
+    apply in_or_app; right; simpl; auto.
+  (* SAnd3 *)
+  - apply_fresh STTyLam as x.
+    unfold open; simpl.
+    eapply STTyApp.
+    rewrite <- open_rec_term.
+    rewrite <- app_nil_r with (l := (x, STTuple (| t1 |) (| t2 |)) :: nil).
+    apply typing_weaken.
+    rewrite app_nil_r.
+    apply IHsub.
+    admit. (* TODO ok rules here *)
+    apply coercions_produce_terms in H.
+    assumption.
+    eapply STTyProj2.
+    apply STTyVar.
+    apply in_or_app; right; simpl; auto.
 Admitted.
+
+Lemma type_correct_terms : forall Gamma E ty, has_type_st Gamma E ty -> STTerm E.
+Proof.
+  intros.
+  induction H.
+  apply STTerm_Var.
+  apply STTerm_Lit.
+  apply_fresh STTerm_Lam as x.
+  apply H0.
+  unfold not; intros; apply Frx; rewrite union_spec; rewrite union_spec; left; left; auto.
+  apply STTerm_App; auto.
+  apply STTerm_Pair; auto.
+  apply STTerm_Proj1; auto.
+  apply STTerm_Proj2; auto.
+Defined.
   
 (* Type preservation: Theorem 1 *)
 Lemma type_preservation : forall x ty E (Gamma : context PTyp) (H : has_type_source Gamma x ty E),
@@ -755,23 +1288,30 @@ Proof.
   induction H; subst.
   (* TyVar *)
   apply STTyVar.
-  now apply exists_persists.
+  now apply in_persists.
   (* TyLit *)
   apply STTyLit.
-  (* TyPair *)
-  Focus 3.
+  (* TyLam *)
   simpl.
-  apply STTyPair; assumption.
+  apply_fresh STTyLam as x.
+  unfold open; simpl.
+  assert (Ha : not (In x L)).
+  unfold not; intros; apply Frx; rewrite union_spec; left; assumption.
+  apply H0 in Ha.
+  unfold conv_context in Ha.
+  simpl in Ha; unfold mapctx in Ha.
+  rewrite map_app in Ha; simpl in *.
+  rewrite <- open_rec_term.
+  assumption.
+  apply type_correct_terms in Ha.
+  assumption.  
   (* TyApp *)
-  Focus 2.
   simpl in *.
   apply STTyApp with (A := |A|).
   assumption.
-  apply type_correct_coercions with (Gamma := ∥ Gamma ∥) in H1.
+  apply type_correct_coercions with (Gamma := (∥ Gamma ∥)) in H1.
   apply STTyApp with (A := |C|); assumption.
-  (* TyLam *)
+  (* TyPair *)
   simpl.
-  apply STTyLam with (L := L).
-  intros.
-  apply H in H1.
-Admitted.
+  apply STTyPair; assumption.
+Defined.
